Phi_Semantics/PhiSem_CF_Basic.thy
@@ -1,7 +1,7 @@
 chapter \<open>Basic Control Flow\<close>
 
 theory PhiSem_CF_Basic
-  imports PhiSem_Generic_Boolean
+  imports PhiSem_Generic_Boolean "HOL-Library.While_Combinator"
 begin
 
 section \<open>Instructions\<close>
@@ -103,6 +103,7 @@ subsubsection \<open>Syntax for Annotations\<close>
 consts Invariant :: \<open>bool \<Rightarrow> bool\<close> ("Inv: _" [100] 36)
 consts Guard :: \<open>bool \<Rightarrow> bool\<close> ("Guard: _" [100] 36)
 consts End   :: \<open>bool \<Rightarrow> bool\<close> ("End: _" [100] 36)
+consts Transition :: \<open>'a \<Rightarrow> bool\<close> ("Transition: _" [100] 36)
 
 subsection \<open>Branch-like\<close>
 
@@ -174,23 +175,6 @@ throws E
   \<medium_left_bracket> B \<medium_right_bracket>.
   \<medium_right_bracket> by simp .
 
-proc while:
-  assumes \<open>\<p>\<a>\<r>\<a>\<m> ( X x \<s>\<u>\<b>\<j> x. Inv: invariant x \<and> Guard: cond x)\<close>
-  assumes V[unfolded Action_Tag_def]:
-           "X' \<i>\<m>\<p>\<l>\<i>\<e>\<s> ((X x \<r>\<e>\<m>\<a>\<i>\<n>\<s> R) \<s>\<u>\<b>\<j> x. invariant x) \<a>\<n>\<d> Any @action ToSA"
-    and C: "\<forall>x. \<p>\<r>\<e>\<m>\<i>\<s>\<e> invariant x \<longrightarrow> \<p>\<r>\<o>\<c> Cond \<lbrace> R\<heavy_comma> X x \<longmapsto> R\<heavy_comma> X x'\<heavy_comma> \<v>\<a>\<l> cond x' \<Ztypecolon> \<bool> \<s>\<u>\<b>\<j> x'. invariant x' \<rbrace> \<t>\<h>\<r>\<o>\<w>\<s> E1"
-    and B: "\<forall>x. \<p>\<r>\<e>\<m>\<i>\<s>\<e> invariant x \<longrightarrow> \<p>\<r>\<e>\<m>\<i>\<s>\<e> cond x \<longrightarrow> \<p>\<r>\<o>\<c> Body \<lbrace> R\<heavy_comma> X x \<longmapsto> R\<heavy_comma> X x' \<s>\<u>\<b>\<j> x'. invariant x' \<rbrace> \<t>\<h>\<r>\<o>\<w>\<s> E2"
-  input  \<open>X'\<close>
-  output \<open>R\<heavy_comma> X x \<s>\<u>\<b>\<j> x. invariant x \<and> \<not> cond x\<close>
-  throws \<open>E1 + E2\<close>
-  \<medium_left_bracket> V C
-    branch \<medium_left_bracket>
-      do_while \<open>R\<heavy_comma> X vars \<s>\<u>\<b>\<j> vars. Inv: invariant vars \<and> Guard: cond vars\<close>
-      \<medium_left_bracket> B C \<medium_right_bracket>.
-      \<medium_right_bracket>.
-    \<medium_left_bracket> \<medium_right_bracket> for \<open>R\<heavy_comma> X vars \<s>\<u>\<b>\<j> vars. invariant vars \<and> \<not> cond vars\<close> ..
-  \<medium_right_bracket> .. .
-
 (*
 We fail to infer the abstraction of the loop guard automatically but
 require users to give by an annotation.
@@ -204,6 +188,45 @@ simplifications like beta reduction,
 causing it is very difficult to recover the actual abstract guard
 \<open>cond\<close> from the reduced composition \<open>cond x'\<close>.
 *)
+
+proc while:
+  assumes \<open>\<p>\<a>\<r>\<a>\<m> ( X x \<s>\<u>\<b>\<j> x. Inv: invariant x \<and> Guard: cond x)\<close>
+  assumes V: "X' \<i>\<m>\<p>\<l>\<i>\<e>\<s> ((X x \<r>\<e>\<m>\<a>\<i>\<n>\<s> R) \<s>\<u>\<b>\<j> x. invariant x) \<a>\<n>\<d> Any @action ToSA"
+    and C: "\<forall>x. \<p>\<r>\<e>\<m>\<i>\<s>\<e> invariant x \<longrightarrow> \<p>\<r>\<o>\<c> Cond \<lbrace> R\<heavy_comma> X x \<longmapsto> R\<heavy_comma> X x'\<heavy_comma> \<v>\<a>\<l> cond x' \<Ztypecolon> \<bool> \<s>\<u>\<b>\<j> x'. invariant x' \<rbrace> \<t>\<h>\<r>\<o>\<w>\<s> E1"
+    and B: "\<forall>x. \<p>\<r>\<e>\<m>\<i>\<s>\<e> invariant x \<longrightarrow> \<p>\<r>\<e>\<m>\<i>\<s>\<e> cond x \<longrightarrow> \<p>\<r>\<o>\<c> Body \<lbrace> R\<heavy_comma> X x \<longmapsto> R\<heavy_comma> X x' \<s>\<u>\<b>\<j> x'. invariant x' \<rbrace> \<t>\<h>\<r>\<o>\<w>\<s> E2"
+  input  \<open>X'\<close>
+  output \<open>R\<heavy_comma> X x \<s>\<u>\<b>\<j> x. invariant x \<and> \<not> cond x\<close>
+  throws \<open>E1 + E2\<close>
+  \<medium_left_bracket> V C
+    branch \<medium_left_bracket>
+      do_while \<open>R\<heavy_comma> X vars \<s>\<u>\<b>\<j> vars. Inv: invariant vars \<and> Guard: cond vars\<close>
+      \<medium_left_bracket> B C \<medium_right_bracket>.
+      \<medium_right_bracket>.
+    \<medium_left_bracket> \<medium_right_bracket> for \<open>R\<heavy_comma> X vars \<s>\<u>\<b>\<j> vars. invariant vars \<and> \<not> cond vars\<close> ..
+  \<medium_right_bracket> .. .
+
+
+proc (nodef) refine_while:
+  assumes \<open>\<p>\<a>\<r>\<a>\<m> ( X x \<s>\<u>\<b>\<j> x. Inv: invariant x \<and> Guard: cond x \<and> Transition: f x)\<close>
+  assumes V: "X' \<i>\<m>\<p>\<l>\<i>\<e>\<s> (X x \<r>\<e>\<m>\<a>\<i>\<n>\<s> R) \<s>\<u>\<b>\<j> invariant x \<a>\<n>\<d> Any @action ToSA"
+    and C: "\<forall>x. \<p>\<r>\<e>\<m>\<i>\<s>\<e> invariant x \<longrightarrow> \<p>\<r>\<o>\<c> Cond \<lbrace> R\<heavy_comma> X x \<longmapsto> R\<heavy_comma> X x\<heavy_comma> \<v>\<a>\<l> cond x \<Ztypecolon> \<bool> \<rbrace> \<t>\<h>\<r>\<o>\<w>\<s> E1"
+    and B: "\<forall>x. \<p>\<r>\<e>\<m>\<i>\<s>\<e> invariant x \<longrightarrow> \<p>\<r>\<e>\<m>\<i>\<s>\<e> cond x \<longrightarrow> \<p>\<r>\<o>\<c> Body \<lbrace> R\<heavy_comma> X x \<longmapsto> R\<heavy_comma> X x' \<s>\<u>\<b>\<j> x'. x' = f x \<and> invariant x' \<rbrace> \<t>\<h>\<r>\<o>\<w>\<s> E2"
+  input \<open>X'\<close>
+  output \<open>R\<heavy_comma> X x' \<s>\<u>\<b>\<j> x'. x' = While_Combinator.while cond f x \<and> invariant x'\<close>
+  throws \<open>E1 + E2\<close>
+  \<medium_left_bracket> V ;;
+    while \<open>X x' \<s>\<u>\<b>\<j> x' i.
+        Inv: (x' = (f ^^ i) x \<and> (\<forall>k < i. cond ((f ^^ k) x)) \<and> (\<forall>k \<le> i. invariant ((f ^^ k) x)) ) \<and>
+        Guard: cond x'\<close>
+    \<medium_left_bracket> C \<medium_right_bracket>.
+    \<medium_left_bracket> B \<medium_right_bracket>
+      apply (of_tac  \<open>\<lambda>_. i + 1\<close>) using \<phi> apply (auto simp add: less_Suc_eq_le)
+      using le_neq_implies_less apply blast
+      by (metis funpow.simps(2) less_Suc_eq_le nat_less_le o_apply) ;;
+  \<medium_right_bracket> using \<phi> apply (auto simp add: While_Combinator.while_def while_option_def)
+    by (metis (mono_tags, lifting) LeastI_ex Least_le le_eq_less_or_eq) .
+
+
 
 
 subsection \<open>Recursion\<close>
