Phi_System/PhiSem_Formalization_Tools.thy
@@ -47,6 +47,11 @@ lemma \<phi>M_assume[intro!]:
   unfolding \<phi>Procedure_def \<phi>M_assume_def bind_def Return_def det_lift_def
   by clarsimp
 
+lemma \<phi>M_assume1[intro!]:
+  \<open>\<p>\<r>\<o>\<c> (\<phi>M_assume P) \<lbrace> Void \<longmapsto> Void \<s>\<u>\<b>\<j> P \<rbrace> \<t>\<h>\<r>\<o>\<w>\<s> E\<close>
+  unfolding \<phi>M_assume_def \<phi>Procedure_def bind_def Return_def det_lift_def
+  by clarsimp
+
 lemma \<phi>M_tail_left:  \<open>\<p>\<r>\<o>\<c> F \<lbrace> 1\<heavy_comma> X \<longmapsto> Y \<rbrace> \<t>\<h>\<r>\<o>\<w>\<s> E \<Longrightarrow> \<p>\<r>\<o>\<c> F \<lbrace> X \<longmapsto> Y \<rbrace> \<t>\<h>\<r>\<o>\<w>\<s> E\<close> by simp
 lemma \<phi>M_tail_right: \<open>\<p>\<r>\<o>\<c> F \<lbrace> X \<longmapsto> \<lambda>v. 1 \<heavy_comma> Y v \<rbrace> \<t>\<h>\<r>\<o>\<w>\<s> E \<Longrightarrow> \<p>\<r>\<o>\<c> F \<lbrace> X \<longmapsto> Y \<rbrace> \<t>\<h>\<r>\<o>\<w>\<s> E\<close> by simp
 lemma \<phi>M_tail_right_right: \<open>\<p>\<r>\<o>\<c> F \<lbrace> X \<longmapsto> \<lambda>v. Y v\<heavy_comma> 1 \<rbrace> \<t>\<h>\<r>\<o>\<w>\<s> E \<Longrightarrow> \<p>\<r>\<o>\<c> F \<lbrace> X \<longmapsto> Y \<rbrace> \<t>\<h>\<r>\<o>\<w>\<s> E\<close> by simp
