Phi_System/Phi_BI.thy
@@ -278,6 +278,7 @@ lemma ExSet_times_right[simp]: "(L * ExSet T) = (\<exists>* c. L * T c)" by (sim
 
 lemma ExSet_simps[simp]:
   \<open>ExSet (\<lambda>_. T) = T\<close>
+  \<open>(\<exists>* x. F x \<s>\<u>\<b>\<j> x = y) = (F y)\<close>
   \<open>(\<exists>* x. F x \<s>\<u>\<b>\<j> x = y \<and> P x) = (F y \<s>\<u>\<b>\<j> P y)\<close>
   \<open>(X b \<s>\<u>\<b>\<j> P b \<s>\<u>\<b>\<j> b. Q b) = (X b \<s>\<u>\<b>\<j> b. P b \<and> Q b)\<close>
   \<open>(X2 a b \<s>\<u>\<b>\<j> a. P2 a b \<s>\<u>\<b>\<j> b. Q b) = (X2 a b \<s>\<u>\<b>\<j> a b. P2 a b \<and> Q b)\<close>
